RM history

io/BugReify.fst
@@ -22,8 +22,8 @@ assume type event **)
 
 type trace = list event
 
-let hist_post a = lt:trace -> r:a -> Type0
-let hist_pre = h:trace -> Type0
+let hist_post a = trace -> r:a -> Type0
+let hist_pre = Type0
 
 let hist0 a = hist_post a -> hist_pre
 
@@ -31,27 +31,27 @@ unfold
 let hist_post_ord (p1 p2:hist_post 'a) = forall lt r. p1 lt r ==> p2 lt r
 
 let hist_wp_monotonic (wp:hist0 'a) =
-  forall p1 p2. (p1 `hist_post_ord` p2) ==> (forall h. wp p1 h ==> wp p2 h)
+  forall p1 p2. (p1 `hist_post_ord` p2) ==> (wp p1 ==> wp p2) 
 
 (** monotonicity seems relevant **)
 let hist a = wp:(hist0 a){hist_wp_monotonic wp}
 
 unfold
 val hist_ord (#a : Type) : hist a -> hist a -> Type0
-let hist_ord wp1 wp2 = forall h p. wp1 p h ==> wp2 p h
+let hist_ord wp1 wp2 = forall p. wp1 p ==> wp2 p
 
 unfold
 let hist_return (x:'a) : hist 'a =
-  fun p _ -> p [] x
+  fun p -> p [] x
 
 unfold
 let hist_bind (#a #b:Type) (w : hist a) (kw : a -> hist b) : hist b =
-  fun p h -> w (fun lt r -> kw r (fun lt' r -> p (lt @ lt') r) (rev lt @ h)) h
+  fun p -> w (fun lt r -> kw r (fun lt' r -> p (lt @ lt') r))
 
 unfold
 let wp_lift_pure_hist (w : pure_wp 'a) : hist 'a =
   FStar.Monotonic.Pure.elim_pure_wp_monotonicity_forall ();
-  fun p _ -> w (p [])
+  fun p -> w (p [])
 
 (** *** Dijkstra Monad **)
 assume val theta : #a:Type -> free a -> hist a
@@ -107,10 +107,10 @@ let test_assert_false
   (t1:Type)
   (t2:Type)
   {| d2:compilable t2 |} 
-  (f:(t1 -> FREEwp (option t2) (fun p h -> (forall r lt. p lt r)))) 
+  (f:(t1 -> FREEwp (option t2) (fun p -> (forall r lt. p lt r)))) 
   (x:t1) : 
   Lemma False =
-  let _ : dm_free (option d2.comp_type) (hist_bind (fun p h -> forall r (lt: trace). p lt r)
+  let _ : dm_free (option d2.comp_type) (hist_bind (fun p -> forall r (lt: trace). p lt r)
                                                    (fun (r:option t2) -> hist_return (compile #_ #(compile_option t2 #d2) r))) =
        reify (compile #_ #(compile_option t2 #d2) (f x)) in
   assert (False)
@@ -120,9 +120,9 @@ let other_tests
   (t1:Type)
   (t2:Type)
   {| d2:compilable t2 |} 
-  (f:(t1 -> FREEwp (option t2) (fun p h -> (forall r lt. p lt r)))) : 
+  (f:(t1 -> FREEwp (option t2) (fun p -> (forall r lt. p lt r)))) : 
   Lemma False =
-  let _ : unit -> FREEwp (option d2.comp_type) (hist_bind (fun p h -> forall r (lt: trace). p lt r)
+  let _ : t1 -> FREEwp (option d2.comp_type) (hist_bind (fun p -> forall r (lt: trace). p lt r)
                                                    (fun (r:option t2) -> hist_return (compile #(option t2) #(compile_option t2 #d2) r))) =
        fun x -> (compile #(option t2) #(compile_option t2 #d2) (f x)) in
   assert (False)
